+++
title = 'kinematics, t0 is zero'
date = '2025-02-17T05:22:18+07:00'
draft = false
type = 'slides'
authors = ['viridi']
tags = ['kinematics']
math = true
url = '25b34'
+++

+ With $a(t) = a$, $v(t_0) = v_0$, $x(t_0) = x_0$, $t_0 \ne 0$, the equations are
{{< fsize "0.95" >}}
$$\tag{H1}
v(t) = v_0 + a(t - t_0),
$$
$$\tag{H2}
x(t) = x_0 + v_0 (t - t_0) +  \tfrac12 a (t - t_0)^2.
$$
{{< /fsize >}}
+ Set $t_0 = 0$, that makes $v(0) = v_0$, $x(0) = x_0$, will turn them into
{{< fsize "0.95" >}}
$$\tag{H3}
v(t) = v_0 + at,
$$
$$\tag{H4}
x(t) = x_0 + v_0 t +  \tfrac12 a t^2.
$$
{{< /fsize >}}
