+++
title = 'the 3rd kine eqns, p2'
date = '2025-02-17T05:52:22+07:00'
draft = false
type = 'slides'
authors = ['viridi']
tags = ['daily-notes']
math = true
url = '25b36'
+++

+ From previous equations following can be obtained
$$\tag{I4}
x = x_0 + v_0 \left( \frac{v - v_0}{a} \right) +  \tfrac12 a \left( \frac{v - v_0}{a} \right)^2.
$$
+ It can be simplified into
$$\tag{I5}
\begin{array}{rcl}
2a(x - x_0) & = & 2v_0 (v - v_0) +  (v - v_0)^2 \newline
& = & (2v_0 + v - v_0)(v - v_0) \newline
& = & (v_0 + v)(v - v_0).
\end{array}
$$
